yui

SemanticswE.v
@@ -2,598 +2,99 @@ Set Implicit Arguments.
 Unset Strict Implicit.
 Set Maximal Implicit Insertion.
 Unset Printing Implicit Defensive.
+Typeclasses eauto := 1.
 
-Require Import ssreflect Basic LAF List Coq.Program.Equality.
+Require Import ssreflect Basic LAF LAFwE Semantics List Coq.Program.Equality.
 
-Variable LAF: LAFs.
+Section SemanticswE.
 
-Section TermSemantics.
-
-  (* A model structure has five basic support sets: 
-- term denotations,
-- valuations (parameterised by a QWorld),
-- label denotations, 
-- positive and negative denotations;
-Then we have
-- an orthogonality relation between negative and positive denotations;
-- a notion of semantic context
-- an interpretation for patterns
-- an interpretation for terms in a valuation in the correct QWorld
-- an interpretation for the reifeied functions 
-   *)
+  Context `(LAFwE: LAFswE).
   
-  Record ModelStructures := 
+  Definition MSwE2MS_base STermsV SLabV SPosV SNegV orthV SContextsV tildV SemTermsV IV
+    :=
+      {|
+        STerms   := STermsV;
+        Valuations := fun qLab: QWorld _ => (qLab:Type) -> STermsV;
+        SLab     := SLabV;
+        SPos     := SPosV;
+        SNeg     := SNegV;
+        orth     := orthV;
+        SContexts := SContextsV;
+        tild     := tildV;
+        SemTerms := SemTermsV;
+        I        := IV
+      |}.
+  
+
+  Class ModelStructureswE
+        {STermsV SLabV SPosV SNegV orthV SContextsV tildV SemTermsV IV}
+    := 
     {
-      STerms   : Type;
-      Valuations : LAF.(QWorld) -> Type;
-      SLab     : Type;
-      SPos     : Type;
-      SNeg     : Type;
-      orth     : SNeg*SPos -> Prop;
-      SContexts: Contexts wextends SLab SNeg STerms Valuations;
-      tild p   : @Dec STerms SLab SNeg (@PatDec LAF p) -> SPos;
-      SemTerms {qLab} : Valuations qLab -> Terms qLab -> STerms;
-      I {w} : SContexts w -> @Reifiable LAF w -> SNeg
+      asMS : SClass (@MSwE2MS_base STermsV SLabV SPosV SNegV 
+                                   orthV SContextsV tildV SemTermsV IV);
+      qLabSem qLab (xq:qLab)(sigma:Valuations (get asMS) qLab) 
+      : SemTerms sigma (asT xq) = sigma xq;
+      reSem qLab qLab' (pi:qLab -> qLab')
+            (r:Terms qLab)(sigma:Valuations (get asMS) qLab'):
+        SemTerms sigma (lift2Terms pi r) = SemTerms ((comp sigma pi):Valuations (get asMS) qLab) r
     }
   .
 
-  Global Arguments tild {_} p _.
+  Canonical MSwE2MS `(ModelStructureswE)
+    := @MSwE2MS_base STermsV SLabV SPosV SNegV orthV SContextsV tildV SemTermsV IV.
 
-  (* A useful abbreviation for semantical decompositions, which will
-  interpret term decompositions *)
-
-  Definition SDec {M} := @Dec M.(STerms) M.(SLab) M.(SNeg).
-
-  (* We now suppose we have a model structure *)
-
-  Variable M: ModelStructures.
-
-  Definition STList := @AList LAF M.(STerms).
-
-  Fixpoint SemTermList qVar sigma l (tl:TList qVar l) :STList l
-    := match tl with
-        | TermNil => TermNil _ _
-        | TermCons so r l' tl' => TermCons so (SemTerms sigma r) (SemTermList sigma tl')
-      end.
-
-  (* The semantics of a negative term is a negative element of the model *)
-  Definition SemN w (rho: M.(SContexts) w) (tm : Neg) := 
-    match tm with
-      | rei f => I rho f
-    end
-  .
-
-  (* The semantics of a TermDec is a SemTree *)
-  Fixpoint SemDec w (rho:M.(SContexts) w) {st} (v : TermDec st) {struct v} :=
-    match v in @TermDec _ _ s return SDec s with
-      | tleafP xp => leafP (readp rho xp)
-      | tleafN tm => leafN (SemN rho tm)
-      | tdummy    => dummy
-      | tnode s1 s2 v1 v2 => node (SemDec rho (st:=s1) v1) (SemDec rho (st:=s2) v2)
-      | tqnode s r v => qnode (SemTerms (readE rho) r) (SemDec rho (st:=s) v)
-    end
-  .
-
-  (* The semantics of a positive term is a positive element of the model *)
-  Definition SemP w (rho:M.(SContexts) w) (pt : Pos) := 
-    match pt with
-        pos p v => tild p (SemDec rho v)
-    end
-  .
-
-  (* The semantics of a command is a pair (negative element,positive
-element) of the model, that may or may not be orthogonal *) 
-
-  Definition SemC w (rho:M.(SContexts) w) (c : Command) :=
-    match c with
-      | cut tm tp => (SemN rho tm,SemP rho tp) 
-      | select xm tp => (rho.(readn) xm,SemP rho tp)
-    end 
-  .
-
-  Definition SemOptionC w (rho:M.(SContexts) w)(oc : OptionCommand) :=
-    match oc with
-      | some c => Some(SemC (rho:M.(SContexts) w) c)
-      | none => None
-    end
-  .
-
-End TermSemantics.
-
-
-
-Section TypeSemantics.
-
-  (************************************************************************)
-  (* We now want to define the semantical interpretation of types/formulae.
-
-This is traditionally done "by induction on types/formulae".
-In our setting, we do not have an inductive structure for types/formulae;
-however, we know how to decompose molecules into atoms and
-molecules.
-
-Morally speaking, this corresponds to accessing sub-formulae, and
-since the sub-formula relation is the well-founded relation that
-allows to define the semantics of formulae, we will now assume the
-well-foundedness of the relation between molecules induced by the
-decomposition relation.
-
-In other words, when a molecule is decomposed into a TypeTree
-according to a pattern, then the molecules belonging to the TypeTree
-have to be SMALLER than the decomposed molecule.
-
-We formalise this. *)
-
-  (* A molecule belongs to a TypeTree, as if it were a set *)
-
-  Inductive  belong l
-  : forall l' st, TypingDec (QST := LAF) st l' -> @Molecule LAF l -> Prop
+  Definition RAwE2RA_base `(MSwE:ModelStructureswE)
+      welfV SemSortsV SemSoCompatV SemAtomV SemAtom_eqV
     :=
-    | rel_leaf  : forall B, belong (TleafN B) B
-    | rel_node1 : forall B l' s1 s2 (t1:TypingDec s1 l') (t2:TypingDec s2 l'),
-                    belong t1 B -> belong (Tnode t1 t2) B
-    | rel_node2 : forall B l' s1 s2 (t1:TypingDec s1 l') (t2:TypingDec s2 l'),  
-                    belong t2 B -> belong (Tnode t1 t2) B
-    | rel_nodeq : forall so B l' s (t:TypingDec s (so::l')), 
-                    belong t B
-                    -> belong (Tqnode t) B
-  .
+    {| 
+      modelStructure := MSwE2MS MSwE;
+      welf := welfV;
+      SemSorts := SemSortsV;
+      SemSoCont := fun qLab Sigma (sigma: Valuations (MSwE2MS MSwE) qLab) 
+                  => forall xq:qLab, SemSortsV (Sigma xq) (sigma xq);
+      SemSoCompat := SemSoCompatV;
+      SemAtom := SemAtomV;
+      SemAtom_eq := SemAtom_eqV
+    |}.
 
-  Inductive relation : DPair (@Molecule LAF) -> DPair (@Molecule LAF) -> Prop :=
-    relation_base:
-      forall p l l' Delta A B, PatternsTyped p Delta A
-                      -> belong Delta B
-                      -> relation (existS _ l B) (existS _ l' A).
-
-  Global Arguments relation_base p {l l'} Delta A B _ _.
-
-  (****************************************************************)
-  (* We now define the semantics of types according to a ModelRaw *)
-
-  Definition Pard {A B M} 
-             (f: forall a:DPair A, STList M (ex1 a) -> B)
-             {qLab} sigma a
-    := f {{ ex1 a, getA (qLab := qLab) a }} (SemTermList sigma (getTerms a)).
-  
-  Record RealisabilityAlg :=
-    { modelStructure :> ModelStructures;
-      welf: well_founded relation;
-      SemSorts : Sorts LAF -> modelStructure.(STerms) -> Prop;
-      SemSoCont qLab: SoContexts qLab -> modelStructure.(Valuations) qLab -> Prop;
-      SemSoCompat qLab: forall Sigma r s sigma, 
-                            SortingRel (qLab := qLab) Sigma r s
-                            -> SemSoCont Sigma sigma
-                            -> SemSorts s (SemTerms sigma r);
-
-      SemAtom : forall a:DPair Atom,
-                STList modelStructure (ex1 a)
-                -> modelStructure.(SLab) -> Prop;
-
-      SemAtom_eq qLab sigma: 
-        forall a b p, is_eq a b
-                 -> Pard (qLab := qLab) (@SemAtom) sigma a p -> Pard (@SemAtom) sigma b p
-
+  Class RealisabilityAlgwE `(MSwE:ModelStructureswE)
+         {welfV SemSortsV SemSoCompatV SemAtomV SemAtom_eqV}
+    :=
+    { 
+      asMSwE := MSwE;
+      asRA := RAwE2RA_base welfV (SemSortsV := SemSortsV) 
+                          SemSoCompatV (SemAtomV := SemAtomV) SemAtom_eqV
     }.
 
-  Global Arguments SemAtom {_} a _ _.
-
-  (* We now assume we have a realisability algebra *)
-
-  Variable M: RealisabilityAlg.
-
-  (* Here is the orthogonal of a set of positive elements of the model, or more precisely a predicate P: M.(positive) -> Prop *)
-  Definition ortho P tm :=
-    forall tp: M.(SPos), P tp -> orth (tm,tp).
-
-  (* Given a molecule A, this is a predicate on positives, that holds if
-this positive is of the form (M.(tild) p v), for some pattern p and
-some SDec v such that p decomposes A into some TypeTree Delta and v is
-in the semantics of Delta. The semantics of TypeTrees not being defined
-yet, it is passed as an argument SemContext.  *)
-
-  Unset Implicit Arguments.
-
-  Inductive PV
-            (A: DPair Molecule)
-            (SemTDec: forall st, TypingDec st (ex1 A)
-                               -> forall tl:STList M (ex1 A), SDec st -> Prop)
-            (tl: STList M (ex1 A))
-  : M.(SPos) -> Prop :=
-    pv : forall p Delta v,
-           PatternsTyped p Delta (ex2 A)
-           -> SemTDec (PatDec p) Delta tl v 
-           -> PV A SemTDec tl (tild p v).
-
-  (* The interpretation (predicate on SDecs) of a TypeTree Delta, given
-a valuation sigma and a function f that provides the negative
-interpretation of any molecule B in Delta *)
-
-  Definition SemTDec_aux
-             (f : forall (A:DPair (@Molecule LAF)), STList M (ex1 A) -> M.(SNeg) -> Prop)
-             l
-             st
-             (Delta : TypingDec (QST := LAF) st l)
-             (tl:STList M l)
-             (v: @SDec M st)
-  : Prop.
-    move : l tl Delta.
-    induction st => l tl Delta; inversion Delta; inversion v.
-    exact (SemAtom {{ l, X }} tl X0).
-    exact (f {{ l, X }} tl X0).
-    exact True.
-    exact (IHst1 X1 l tl X /\ IHst2 X2 l tl X0).
-    exact (SemSorts so X0 /\ IHst X1 (so::l) (TermCons so X0 tl) X).
-  Defined.
-
-
-  (* The positive interpretation (predicate on positives) of a molecule
-A, given a valuation sigma that provides the positive interpretation of
-every molecule variable, and a function f that already provides the
-positive interpretation of any molecule B smaller than A *)
-
-  Definition SemPos_aux
-             (A: DPair Molecule)
-             (f : forall B, relation B A -> STList M (ex1 B) -> M.(SPos) -> Prop)
-    := PV A (SemTDec_aux (fun B tl tm => exists h:relation B A, ortho (f B h tl) tm) (ex1 A)).
-
-  (* The positive interpretation (predicate on positives) of a molecule
-A, given a type valuation sigma. Fixpoint of the previous function, built on
-the well-founded relation on molecules. *)
-
-  Definition SemPos := Fix M.(welf) _ (SemPos_aux).
-
-  (* The negative interpretation (predicate on negatives) of a molecule
-A, given a valuation sigma. It is built as the orthogonal of the positive
-interpretation of A.  *)
-
-  Definition SemNeg A tl := ortho (SemPos A tl).
-
-  (* A new version of the interpretation (predicate on SDecs) of a
-TypeTree Delta, given a valuation sigma, but this time the predicate
-used as the negative interpretation of any molecule B in Delta is not
-passed as a parameter, it is the actual interpretation SemNeg *)
-
-  Definition SemTDec {l st} := SemTDec_aux (@SemNeg) l st.
-
-  (* The definition of SemPos is so far quite cryptic, because of the
-induction that was necessary for the definition to be sound. The
-theorem below characterise SemPos in a much more intuitive way, but
-before that we need the following two lemmas. *)
-
-  Lemma F_ext_aux:
-    forall (x:DPair Molecule)
-      (f g: forall y:DPair Molecule, 
-              relation y x -> STList M (ex1 y) -> M.(SPos) -> Prop),
-      (forall (y:DPair Molecule) (p:relation y x) tl d, f y p tl d <-> g y p tl d) 
-      -> forall st l (Delta:TypingDec st l),
-          forall tl' (v : SDec st),
-            SemTDec_aux (fun (B : DPair Molecule) tl (tm : M.(SNeg)) =>
-                           exists h : relation B x, ortho (f B h tl) tm)
-                        _ _ Delta tl' v ->
-            SemTDec_aux (fun (B : DPair Molecule) tl (tm : M.(SNeg)) =>
-                           exists h : relation B x, ortho (g B h tl) tm)
-                        _ _ Delta tl' v .
-  Proof.
-    move => A f g H st.
-
-    induction st;
-      dependent induction v;
-      dependent induction Delta => //;simpl.
-
-    unfold ortho.
-    elim => h H1.
-    exists h.
-    move => // tp H2.
-    apply: H1.
-    by apply H.
-
-    case => H1 H2.
-    by split; [apply: IHst1 |apply: IHst2].
-
-    clear  IHv.
-    move => [H1 H2].
-    split =>//.
-    by apply IHst.
-  Qed.
-
-  Lemma F_ext :
-    forall (x:DPair Molecule)
-      (f g: forall y:DPair Molecule, 
-              relation y x -> STList M (ex1 y) -> M.(SPos) -> Prop),
-      (forall (y:DPair Molecule) (p:relation y x) tl d, f y p tl d <-> g y p tl d) 
-      -> forall tl d, SemPos_aux x f tl d -> SemPos_aux x g tl d.
-  Proof.
-    move => A f g H tl d.
-    unfold SemPos_aux.
-    elim.
-    intros.
-    apply (pv A _ tl p Delta v) => //.
-    move : v H1 ; clear H0 d.
-    apply F_ext_aux =>//. 
-  Qed.
-
-  Lemma Fix_F_inv :
-    forall (x:DPair Molecule) tl d (r s:Acc relation x),
-      Fix_F (fun A => STList M (ex1 A) -> M.(SPos) -> Prop) 
-            SemPos_aux r tl d 
-      <-> 
-      Fix_F (fun A => STList M (ex1 A) -> M.(SPos) -> Prop)
-            SemPos_aux s tl d.
-  Proof.
-    move => A; induction (M.(welf) A).
-    move => tl d r s.
-    rewrite <- (Fix_F_eq _ _ r). 
-    rewrite <- (Fix_F_eq _ _ s).
-    split.
-    apply (@F_ext _ 
-                 (fun (y : DPair Molecule) (p : relation y x)  =>
-                    Fix_F _ (@SemPos_aux) (Acc_inv r p))) => //=.
-    auto.
-    apply (@F_ext _
-                 (fun (y : DPair Molecule) (p : relation y x)  =>
-                    Fix_F _ (@SemPos_aux) (Acc_inv s p))) => //=.
-    auto.
-  Qed.
-
-  (* Characterisation of SemPos: The first step is to have a
-reformulation that looks much more like the definition of SemPos_aux,
-but with the actual SemPos taking the place of the parameter f *)
-
-  Lemma SemPos_Fix :
-    forall A tl tp, 
-      SemPos A tl tp 
-      <-> PV A 
-           (SemTDec_aux (fun B tl' tm => exists h:relation B A, ortho (SemPos B tl') tm) (ex1 A))
-           tl
-           tp.
-  Proof.
-    move => A tl tp; unfold SemPos; unfold Fix in |- *.
-    rewrite <- Fix_F_eq.
-    split; apply F_ext; intros; apply Fix_F_inv.
-  Qed.
-
-  (* Characterisation of SemPos: The second step is to have a
-reformulation which drops the requirement B smaller than A in its use
-of SemTDec_aux (that requirement was needed for the well-foundedness
-of the definition of SemPos) *)
-
-  Lemma SemPosDec_aux1 : 
-    forall A st l (Delta:TypingDec st l) tl (v:SDec st), 
-      (forall B : DPair Molecule, belong Delta (ex2 B) -> relation B A)
-      -> SemTDec_aux (fun (B : DPair Molecule) tl' (tm : M.(SNeg)) => 
-                       ortho (SemPos B tl') tm) 
-                    l st Delta tl v      
-      -> SemTDec_aux (fun (B : DPair Molecule) tl' (tm : M.(SNeg)) =>
-                       exists _ : relation B A, ortho (SemPos B tl') tm)
-                    l st Delta tl v.
-  Proof.
-    move => A.
-    induction st;
-      dependent induction Delta ; move => tl v; 
-      dependent induction v => H //; simpl.
-
-      + move => H1.
-        assert (belong (TleafN m) m).
-        apply rel_leaf.
-        assert (relation (existS _ l m) A).
-        apply H => //=.
-        by exists H2.
-      + clear IHDelta1 IHDelta2 IHv1 IHv2.
-        elim => H3 H4.
-        split.
-        * apply IHst1 => //.
-          move => B H5.
-          apply: H.
-          apply: rel_node1 => //.
-        * apply: IHst2 => //.
-          move => B H5.
-          apply: H.
-          apply: rel_node2 => //.
-    + clear IHDelta IHv.
-        move => [H1 H2].
-        split =>//.
-        apply: IHst => //.
-        move => B H5.
-        apply: H.
-        apply: rel_nodeq => //.
-    Qed.
-
-  Lemma SemPosDec_aux2: 
-    forall A st l (Delta:TypingDec st l) tl (v:SDec st), 
-      SemTDec_aux (fun (B : DPair Molecule) tl' (tm : M.(SNeg)) =>
-                       exists _ : relation B A, ortho (SemPos B tl') tm)
-                    l st Delta tl v
-      -> SemTDec_aux (fun (B : DPair Molecule) tl' (tm : M.(SNeg)) =>
-                       ortho (SemPos B tl') tm) 
-                    l st Delta tl v.
-  Proof.
-    move => A.
-    induction st;
-      dependent induction Delta ; move => tl v; 
-      dependent induction v => //; simpl.
-    + by move => [_ H] //=.
-    + by elim => H3 H4; split; [ apply IHst1 | apply IHst2].
-    + by move => [H4 H]; split => //; apply: IHst.
-    Qed.
-
-  Lemma SemPosDec_aux: 
-    forall A tl tp, 
-      PV A 
-         (SemTDec_aux (fun B tl' tm => ortho (SemPos B tl') tm) (ex1 A))
-         tl
-         tp      
-      <-> PV A 
-           (SemTDec_aux (fun B tl' tm => exists h:relation B A, ortho (SemPos B tl') tm) (ex1 A))
-           tl
-           tp.
-  Proof.
-    elim => lA Araw.
-    intros.
-    split => H;elim H;clear H;intros; apply (pv {{ lA,Araw }} _ tl p Delta v) => //=.
-    + assert  (forall (B : DPair Molecule),
-                 belong Delta (ex2 B) -> relation B {{ lA,Araw }}).
-        * elim => lB Braw.
-          intros.
-          apply (relation_base p Delta) => //=.
-      apply SemPosDec_aux1 =>//.
-      apply (SemPosDec_aux2 {{ lA,Araw }}) =>//.
-  Qed.
-
-
-  (* Characterisation of SemPos: the final step is to write the
-definition we would actually like, and notice that, when unfolded, it
-is equivalent to the actual definition by using the previous two
-lemmas *)
-
-  Theorem SemPosDec : forall A tl tp, SemPos A tl tp <-> PV A (@SemTDec (ex1 A)) tl tp.
-  Proof.
-    intros;split; intro.
-    apply SemPosDec_aux;apply SemPos_Fix => //=.
-    apply SemPos_Fix;apply SemPosDec_aux => //=.
-  Qed.
-
-  (* We define the interpretation of a typing context as a predicate on
-semantic contexts *)
-
-  Definition SemCont {w}: TContext w -> M.(SContexts) w -> Prop
-    := fun Gamma rho =>
-      SemSoCont (TreadE Gamma) (readE rho)
-      /\ (forall xp, (Pard SemAtom (readE rho)) (Treadp Gamma xp) (readp rho xp))
-      /\ (forall xn, (Pard SemNeg (readE rho)) (Treadn Gamma xn) (readn rho xn)).
-
-End TypeSemantics.
-
-Arguments SemAtom {_} _ _ _.
-Arguments SemPos {M} _ _ _.
-Arguments SemTDec {M l st} _ _ _.
-Arguments SemNeg {M} _ _ _.
-Arguments SemCont {M w} _ _.
-
-Set Implicit Arguments.
-Unset Strict Implicit.
-Set Maximal Implicit Insertion.
-
-(**************************************)
-
-Section Adequacy.
+  Coercion asMSwE: RealisabilityAlgwE >-> ModelStructureswE.
+  Canonical RAwE2RA `(RAwE:RealisabilityAlgwE)
+    := RAwE2RA_base welfV SemSoCompatV SemAtom_eqV.
   
-  (* Even though we don't need to formalise a notion of reduction for
-proof-terms, the Adequacy Lemma requires from a model that its
-orthogonality relation be closed "under anti-reduction" *)
+  Definition TypingCorrwE_Prop `{M: RealisabilityAlgwE} :=
+    forall qLab sigma, GenericCorr
+                (Context1 := TCV qLab)
+                (Context2 := SContexts _)
+                SemSorts
+                (Pard SemAtom sigma)
+                (Pard (SemNeg (M:= RAwE2RA M)) sigma).
 
-  Record FullModel := 
+  Record FullModelwE `{M: RealisabilityAlgwE} := 
     {
-      M0 :> RealisabilityAlg;
-
-      TypingCorr w st :
-        forall (rho:M0.(SContexts) w) Gamma l (Delta:TypingDec st l) tl v, 
-          SemCont Gamma rho
-          -> SemTDec Delta (SemTermList (readE rho) tl) v
-          -> SemCont (Textends [Delta,tl] Gamma) (extends v rho);
-
-      Stability w :
-        forall (f: Reifiable w) (rho: M0.(SContexts) w) (p: Patterns LAF)
-          l Delta (tl:STList M0 l) (v: SDec (PatDec p)) c,
+      asRAwE := M;
+      TypingCorrwE : TypingCorrwE_Prop;
+      StabilitywE w :
+        forall (f: Reifiable w) (rho: SContexts (RAwE2RA M) w) (p: Patterns (LAFwE2LAF LAFwE))
+          l Delta (tl:STList (RAwE2RA M) l) (v: SDec (PatDec p)) c,
           f p =cis= c
           -> SemTDec Delta tl v
           -> orth (SemC (extends v rho) c)
           -> orth (I rho f, tild p v)
     }.
 
-  (* Here is finally the Adequacy Lemma *)
+  Coercion asRAwE: FullModelwE >-> RealisabilityAlgwE.
 
-  Theorem adequacy (M:FullModel) :
-    forall (w:World LAF) (Gamma:TContext w),
-      (forall pt A,
-         PosTyping Gamma pt A
-         ->  forall rho:M.(SContexts) w, SemCont Gamma rho
-                 -> Pard SemPos (readE rho) A (SemP rho pt)
-      )
-      /\ (forall l st (v:TermDec st) Delta tl,
-           DecTyping Gamma v Delta tl
-           ->  forall rho:M.(SContexts) w, SemCont Gamma rho
-                   -> SemTDec (l:=l) Delta (SemTermList (readE rho) tl) (SemDec rho v)
-        )
-      /\ (forall nt A,
-           NegTyping Gamma nt A
-           ->  forall rho:M.(SContexts) w, SemCont Gamma rho
-                   -> Pard SemNeg (readE rho) A (SemN rho nt)
-        )
-      /\ (forall c,
-           OptionCommandTyping Gamma c
-           ->  forall rho:M.(SContexts) w, SemCont Gamma rho
-                   -> exists csem, (SemOptionC rho c) = Some csem /\ orth csem)
-      /\ (forall c,
-           CommandTyping Gamma c
-           ->  forall rho:M.(SContexts) w, SemCont Gamma rho
-                   -> orth (SemC rho c))
-  .
-  Proof.
+End SemanticswE.
 
-    apply typing_ind;intros;
-    [
-      (* Typing a positive *)
-      apply SemPosDec; by apply (pv _ {{l, A}} _ _ p Delta) =>//; apply (H rho H0)
-
-      (* Typing a positive leaf of Sub *)
-      | unfold SemTDec => //= ;
-        by apply (SemAtom_eq i) => //;
-        elim: H => _ [H _]; apply:H
-
-      (* Typing a negative leaf of Sub *)
-      | unfold SemTDec => //= ; by apply H
-
-      (* Typing a dummy leaf of Sub *)
-      | unfold SemTDec => //= 
-
-      (* Typing a node of Sub *)
-      | by unfold SemTDec => //=; unfold SemTDec in H, H0; split; [apply H|apply H0]
-
-      (* Typing a qnode of Sub *)
-      | unfold SemTDec => //=; 
-        by split;
-           [ apply (SemSoCompat (Sigma:=TreadE Gamma)); move:H0;rewrite/SemCont;elim => H2 _ 
-           | apply H ]
-
-      (* Typing a negative *)
-      | 
-
-      (* Typing an optional command *)
-      | by exists (SemC rho c); split; [| apply: H]
-
-      (* Typing a cut *)
-      | by rewrite /SemTDec/Pard/SemNeg/ortho/getA/getTerms in H;apply H =>//; apply H0
-
-      (* Typing a select *)
-      | by rewrite /SemC/SemCont/Pard/SemNeg/ortho in H0;apply H0;apply H
-    ].
-
-    (* Typing a negative *)
-    rewrite /Pard/SemNeg/ortho/getA/getTerms => /= tp H1.
-    assert (PV M {{ l,A }} (@SemTDec M l) (SemTermList (readE rho) tl) tp)
-      by apply SemPosDec =>//=.
-    elim H2 => /= p Delta v H3 H4; clear H2.
-    have H6: (exists csem : SNeg M * SPos M,
-                SemOptionC (extends v rho) (f p) = Some csem
-                /\ orth csem).
-    apply: (H p Delta) => //.
-    apply: TypingCorr => //.
-    elim: H6 => csem [H7 H8].
-    have : exists c, (f p = some c).
-    move : H7.
-    elim (f p) =>/=.
-    by move => c _; exists c.
-    move => H9;discriminate H9.
-    elim => c H9.
-    apply (Stability (Delta := Delta) (tl := (SemTermList (readE rho) tl)) (c := c)) => //.
-    by rewrite H9.
-    move:H7.
-    rewrite H9 => /= H7; injection H7; clear H7 => H7; rewrite H7 =>//.
-  Qed.
-
-End Adequacy.
-
-Print Assumptions adequacy.
 
 (* Lemma SemTermListRen {QVar QVar'}: *)
 (*       forall (ren:QVar -> QVar') (sigma:@qvaluation M QVar) tau, *)
@@ -652,6 +153,10 @@ Print Assumptions adequacy.
 (*     rewrite /Pard/ParRen/ex1/getA/getTerms/ex2; simpl. *)
 (*     rewrite (SemTermListRen (QVar := w.(QVar)) (QVar' := w'.(QVar)) M ren sigma tau) =>//. *)
 (* Qed. *)
+
+
+
+
 
 (* apply (SemPos2Treelift _ _ rho.(readq) _ (qinject Context (PatTree p) w) (PatTree p) (qnew Context (PatTree p) w) l Delta (SemTermList M rho.(readq) tl) (UTTermListRen (qinject Context (PatTree p) w) tl))=> // . *)
 (* move => xq. *)
